Prove theorems up to and including Uctor_rename

operations/Recursor.thy
@@ -37,15 +37,15 @@ consts U2ctor :: "('var::{var_T1_pre,var_T2_pre}, 'tyvar::{var_T1_pre,var_T2_pre
 axiomatization where
   (* parameter axioms *)
     Pmap_id0: "Pmap id id = id"
-and Pmap_comp0: "bij f1 \<Longrightarrow> |supp (f1::'var::{var_T1_pre,var_T2_pre} \<Rightarrow> 'var)| <o |UNIV::'var set| \<Longrightarrow> bij f2 \<Longrightarrow> |supp (g2::'tyvar::{var_T1_pre,var_T2_pre} \<Rightarrow> 'tyvar)| <o |UNIV::'tyvar set| \<Longrightarrow>
+and Pmap_comp0: "bij f1 \<Longrightarrow> |supp (f1::'var::{var_T1_pre,var_T2_pre} \<Rightarrow> 'var)| <o |UNIV::'var set| \<Longrightarrow> bij f2 \<Longrightarrow> |supp (f2::'tyvar::{var_T1_pre,var_T2_pre} \<Rightarrow> 'tyvar)| <o |UNIV::'tyvar set| \<Longrightarrow>
   bij g1 \<Longrightarrow> |supp (g1::'var \<Rightarrow> 'var)| <o |UNIV::'var set| \<Longrightarrow> bij g2 \<Longrightarrow> |supp (g2::'tyvar \<Rightarrow> 'tyvar)| <o |UNIV::'tyvar set| \<Longrightarrow>
   Pmap (g1 \<circ> f1) (g2 \<circ> f2) = Pmap g1 g2 \<circ> Pmap f1 f2"
-and Pmap_cong_id: "bij f1 \<Longrightarrow> |supp (f1::'var::{var_T1_pre,var_T2_pre} \<Rightarrow> 'var)| <o |UNIV::'var set| \<Longrightarrow> bij f2 \<Longrightarrow> |supp (g2::'tyvar::{var_T1_pre,var_T2_pre} \<Rightarrow> 'tyvar)| <o |UNIV::'tyvar set| \<Longrightarrow>
-  (\<And>a. a \<in> PFVars_1 d \<Longrightarrow> f1 a = a) \<Longrightarrow> (\<And>b. b \<in> PFVars_2 d \<Longrightarrow> f2 a = a) \<Longrightarrow>
+and Pmap_cong_id: "bij f1 \<Longrightarrow> |supp (f1::'var::{var_T1_pre,var_T2_pre} \<Rightarrow> 'var)| <o |UNIV::'var set| \<Longrightarrow> bij f2 \<Longrightarrow> |supp (f2::'tyvar::{var_T1_pre,var_T2_pre} \<Rightarrow> 'tyvar)| <o |UNIV::'tyvar set| \<Longrightarrow>
+  (\<And>a. a \<in> PFVars_1 d \<Longrightarrow> f1 a = a) \<Longrightarrow> (\<And>a. a \<in> PFVars_2 d \<Longrightarrow> f2 a = a) \<Longrightarrow>
   Pmap f1 f2 d = d"
-and PFVars_Pmap_1: "bij f1 \<Longrightarrow> |supp (f1::'var::{var_T1_pre,var_T2_pre} \<Rightarrow> 'var)| <o |UNIV::'var set| \<Longrightarrow> bij f2 \<Longrightarrow> |supp (g2::'tyvar::{var_T1_pre,var_T2_pre} \<Rightarrow> 'tyvar)| <o |UNIV::'tyvar set| \<Longrightarrow>
+and PFVars_Pmap_1: "bij f1 \<Longrightarrow> |supp (f1::'var::{var_T1_pre,var_T2_pre} \<Rightarrow> 'var)| <o |UNIV::'var set| \<Longrightarrow> bij f2 \<Longrightarrow> |supp (f2::'tyvar::{var_T1_pre,var_T2_pre} \<Rightarrow> 'tyvar)| <o |UNIV::'tyvar set| \<Longrightarrow>
   PFVars_1 (Pmap f1 f2 d) = f1 ` PFVars_1 d"
-and PFVars_Pmap_2: "bij f1 \<Longrightarrow> |supp (f1::'var::{var_T1_pre,var_T2_pre} \<Rightarrow> 'var)| <o |UNIV::'var set| \<Longrightarrow> bij f2 \<Longrightarrow> |supp (g2::'tyvar::{var_T1_pre,var_T2_pre} \<Rightarrow> 'tyvar)| <o |UNIV::'tyvar set| \<Longrightarrow>
+and PFVars_Pmap_2: "bij f1 \<Longrightarrow> |supp (f1::'var::{var_T1_pre,var_T2_pre} \<Rightarrow> 'var)| <o |UNIV::'var set| \<Longrightarrow> bij f2 \<Longrightarrow> |supp (f2::'tyvar::{var_T1_pre,var_T2_pre} \<Rightarrow> 'tyvar)| <o |UNIV::'tyvar set| \<Longrightarrow>
   PFVars_2 (Pmap f1 f2 d) = f2 ` PFVars_2 d"
 and small_PFVars_1: "|PFVars_1 d| <o |UNIV::'var set|"
 and small_PFVars_2: "|PFVars_2 d| <o |UNIV::'tyvar set|"
@@ -53,69 +53,68 @@ and small_avoiding_set1: "|avoiding_set1::'var set| <o |UNIV::'var set|"
 and small_avoiding_set2: "|avoiding_set2::'tyvar set| <o |UNIV::'tyvar set|"
   (* model 1 axioms *)
 and U1map_id0: "U1map id id (t1::('var, 'tyvar, 'a, 'b) T1) = id"
-and U1map_comp0: "bij f1 \<Longrightarrow> |supp (f1::'var::{var_T1_pre,var_T2_pre} \<Rightarrow> 'var)| <o |UNIV::'var set| \<Longrightarrow> bij f2 \<Longrightarrow> |supp (g2::'tyvar::{var_T1_pre,var_T2_pre} \<Rightarrow> 'tyvar)| <o |UNIV::'tyvar set| \<Longrightarrow>
+and U1map_comp0: "bij f1 \<Longrightarrow> |supp (f1::'var::{var_T1_pre,var_T2_pre} \<Rightarrow> 'var)| <o |UNIV::'var set| \<Longrightarrow> bij f2 \<Longrightarrow> |supp (f2::'tyvar::{var_T1_pre,var_T2_pre} \<Rightarrow> 'tyvar)| <o |UNIV::'tyvar set| \<Longrightarrow>
   bij g1 \<Longrightarrow> |supp (g1::'var \<Rightarrow> 'var)| <o |UNIV::'var set| \<Longrightarrow> bij g2 \<Longrightarrow> |supp (g2::'tyvar \<Rightarrow> 'tyvar)| <o |UNIV::'tyvar set| \<Longrightarrow>
   U1map (g1 \<circ> f1) (g2 \<circ> f2) t1 = U1map g1 g2 t1 \<circ> U1map f1 f2 t1"
-and U1map_cong_id: "bij f1 \<Longrightarrow> |supp (f1::'var::{var_T1_pre,var_T2_pre} \<Rightarrow> 'var)| <o |UNIV::'var set| \<Longrightarrow> bij f2 \<Longrightarrow> |supp (g2::'tyvar::{var_T1_pre,var_T2_pre} \<Rightarrow> 'tyvar)| <o |UNIV::'tyvar set| \<Longrightarrow>
-  (\<And>a. a \<in> U1FVars_1 t1 u1 \<Longrightarrow> f1 a = a) \<Longrightarrow> (\<And>b. b \<in> U1FVars_2 t1 u1 \<Longrightarrow> f2 a = a) \<Longrightarrow>
+and U1map_cong_id: "bij f1 \<Longrightarrow> |supp (f1::'var::{var_T1_pre,var_T2_pre} \<Rightarrow> 'var)| <o |UNIV::'var set| \<Longrightarrow> bij f2 \<Longrightarrow> |supp (f2::'tyvar::{var_T1_pre,var_T2_pre} \<Rightarrow> 'tyvar)| <o |UNIV::'tyvar set| \<Longrightarrow>
+  (\<And>a. a \<in> U1FVars_1 t1 u1 \<Longrightarrow> f1 a = a) \<Longrightarrow> (\<And>a. a \<in> U1FVars_2 t1 u1 \<Longrightarrow> f2 a = a) \<Longrightarrow>
   U1map f1 f2 t1 u1 = u1"
-and U1FVars_Umap_1: "bij f1 \<Longrightarrow> |supp (f1::'var::{var_T1_pre,var_T2_pre} \<Rightarrow> 'var)| <o |UNIV::'var set| \<Longrightarrow> bij f2 \<Longrightarrow> |supp (g2::'tyvar::{var_T1_pre,var_T2_pre} \<Rightarrow> 'tyvar)| <o |UNIV::'tyvar set| \<Longrightarrow>
+and U1FVars_Umap_1: "bij f1 \<Longrightarrow> |supp (f1::'var::{var_T1_pre,var_T2_pre} \<Rightarrow> 'var)| <o |UNIV::'var set| \<Longrightarrow> bij f2 \<Longrightarrow> |supp (f2::'tyvar::{var_T1_pre,var_T2_pre} \<Rightarrow> 'tyvar)| <o |UNIV::'tyvar set| \<Longrightarrow>
   U1FVars_1 (rrename_T1 f1 f2 t1) (U1map f1 f2 t1 u1) = f1 ` U1FVars_1 t1 u1"
-and U1FVars_Umap_2: "bij f1 \<Longrightarrow> |supp (f1::'var::{var_T1_pre,var_T2_pre} \<Rightarrow> 'var)| <o |UNIV::'var set| \<Longrightarrow> bij f2 \<Longrightarrow> |supp (g2::'tyvar::{var_T1_pre,var_T2_pre} \<Rightarrow> 'tyvar)| <o |UNIV::'tyvar set| \<Longrightarrow>
+and U1FVars_Umap_2: "bij f1 \<Longrightarrow> |supp (f1::'var::{var_T1_pre,var_T2_pre} \<Rightarrow> 'var)| <o |UNIV::'var set| \<Longrightarrow> bij f2 \<Longrightarrow> |supp (f2::'tyvar::{var_T1_pre,var_T2_pre} \<Rightarrow> 'tyvar)| <o |UNIV::'tyvar set| \<Longrightarrow>
   U1FVars_2 (rrename_T1 f1 f2 t1) (U1map f1 f2 t1 u1) = f2 ` U1FVars_2 t1 u1"
-and U1map_Uctor: "bij f1 \<Longrightarrow> |supp (f1::'var::{var_T1_pre,var_T2_pre} \<Rightarrow> 'var)| <o |UNIV::'var set| \<Longrightarrow> bij f2 \<Longrightarrow> |supp (g2::'tyvar::{var_T1_pre,var_T2_pre} \<Rightarrow> 'tyvar)| <o |UNIV::'tyvar set| \<Longrightarrow>
+and U1map_Uctor: "bij f1 \<Longrightarrow> |supp (f1::'var::{var_T1_pre,var_T2_pre} \<Rightarrow> 'var)| <o |UNIV::'var set| \<Longrightarrow> bij f2 \<Longrightarrow> |supp (f2::'tyvar::{var_T1_pre,var_T2_pre} \<Rightarrow> 'tyvar)| <o |UNIV::'tyvar set| \<Longrightarrow>
   U1map f1 f2 (T1_ctor (map_T1_pre id id id id id id fst fst fst fst y)) (U1ctor y p)
 = U1ctor (map_T1_pre f1 f2 id id f1 f2
-    (\<lambda>(t, pu). (rrename_T1 f1 f2 t, \<lambda>p. U1map f1 f2 t (pu p)))
-    (\<lambda>(t, pu). (rrename_T1 f1 f2 t, \<lambda>p. U1map f1 f2 t (pu p)))
-    (\<lambda>(t, pu). (rrename_T2 f1 f2 t, \<lambda>p. U2map f1 f2 t (pu p)))
-    (\<lambda>(t, pu). (rrename_T2 f1 f2 t, \<lambda>p. U2map f1 f2 t (pu p)))
+    (\<lambda>(t, pu). (rrename_T1 f1 f2 t, \<lambda>p. U1map f1 f2 t (pu (Pmap (inv f1) (inv f2) p))))
+    (\<lambda>(t, pu). (rrename_T1 f1 f2 t, \<lambda>p. U1map f1 f2 t (pu (Pmap (inv f1) (inv f2) p))))
+    (\<lambda>(t, pu). (rrename_T2 f1 f2 t, \<lambda>p. U2map f1 f2 t (pu (Pmap (inv f1) (inv f2) p))))
+    (\<lambda>(t, pu). (rrename_T2 f1 f2 t, \<lambda>p. U2map f1 f2 t (pu (Pmap (inv f1) (inv f2) p))))
  y) (Pmap f1 f2 p)"
 and U1FVars_subset_1: "set5_T1_pre (y::(_, _, 'a::{var_T1_pre,var_T2_pre}, 'b, _, _, _, _, _, _) T1_pre) \<inter> (PFVars_1 p \<union> avoiding_set1) = {} \<Longrightarrow>
-  (\<And>t pu p. (t, pu) \<in> set7_T1_pre y \<Longrightarrow> U1FVars_1 t (pu p) \<subseteq> FFVars_T11 t \<union> PFVars_1 p \<union> avoiding_set1) \<Longrightarrow>
-  (\<And>t pu p. (t, pu) \<in> set8_T1_pre y \<Longrightarrow> U1FVars_1 t (pu p) - set5_T1_pre y \<subseteq> FFVars_T11 t - set5_T1_pre y \<union> PFVars_1 p \<union> avoiding_set1) \<Longrightarrow>
-  (\<And>t pu p. (t, pu) \<in> set9_T1_pre y \<Longrightarrow> U2FVars_1 t (pu p) \<subseteq> FFVars_T21 t \<union> PFVars_1 p \<union> avoiding_set1) \<Longrightarrow>
-  (\<And>t pu p. (t, pu) \<in> set10_T1_pre y \<Longrightarrow> U2FVars_1 t (pu p) - set5_T1_pre y \<subseteq> FFVars_T21 t - set5_T1_pre y \<union> PFVars_1 p \<union> avoiding_set1) \<Longrightarrow>
-  U1FVars_1 (T1_ctor (map_T1_pre id id id id id id fst fst fst fst y)) (U1ctor y p) \<subseteq> FFVars_T11 (T1_ctor (map_T1_pre id id id id id id fst fst fst fst y)) \<union> set1_T1_pre y \<union> PFVars_1 p"
-and U1FVars_subset_2: "set6_T1_pre y \<inter> (PFVars_2 p \<union> avoiding_set2) = {} \<Longrightarrow>
-  (\<And>t pu p. (t, pu) \<in> set7_T1_pre y \<Longrightarrow> U1FVars_2 t (pu p) \<subseteq> FFVars_T12 t \<union> PFVars_2 p \<union> avoiding_set2) \<Longrightarrow>
-  (\<And>t pu p. (t, pu) \<in> set8_T1_pre y \<Longrightarrow> U1FVars_2 t (pu p) - set6_T1_pre y \<subseteq> FFVars_T12 t - set6_T1_pre y \<union> PFVars_2 p \<union> avoiding_set2) \<Longrightarrow>
-  (\<And>t pu p. (t, pu) \<in> set9_T1_pre y \<Longrightarrow> U2FVars_2 t (pu p) \<subseteq> FFVars_T22 t \<union> PFVars_2 p \<union> avoiding_set2) \<Longrightarrow>
-  (\<And>t pu p. (t, pu) \<in> set10_T1_pre y \<Longrightarrow> U2FVars_2 t (pu p) \<subseteq> FFVars_T22 t \<union> PFVars_2 p \<union> avoiding_set2) \<Longrightarrow>
-  U1FVars_2 (T1_ctor (map_T1_pre id id id id id id fst fst fst fst y)) (U1ctor y p) \<subseteq> FFVars_T12 (T1_ctor (map_T1_pre id id id id id id fst fst fst fst y)) \<union> set2_T1_pre y \<union> PFVars_2 p"
+  (\<And>t pu p. (t, pu) \<in> set7_T1_pre y \<union> set8_T1_pre y \<Longrightarrow> U1FVars_1 t (pu p) \<subseteq> FFVars_T11 t \<union> PFVars_1 p \<union> avoiding_set1) \<Longrightarrow>
+  (\<And>t pu p. (t, pu) \<in> set9_T1_pre y \<union> set10_T1_pre y \<Longrightarrow> U2FVars_1 t (pu p) \<subseteq> FFVars_T21 t \<union> PFVars_1 p \<union> avoiding_set1) \<Longrightarrow>
+  U1FVars_1 (T1_ctor (map_T1_pre id id id id id id fst fst fst fst y)) (U1ctor y p) \<subseteq> FFVars_T11 (T1_ctor (map_T1_pre id id id id id id fst fst fst fst y)) \<union> PFVars_1 p \<union> avoiding_set1"
+and U1FVars_subset_2: "set6_T1_pre (y::(_, _, 'a::{var_T1_pre,var_T2_pre}, 'b, _, _, _, _, _, _) T1_pre) \<inter> (PFVars_2 p \<union> avoiding_set2) = {} \<Longrightarrow>
+  (\<And>t pu p. (t, pu) \<in> set7_T1_pre y \<union> set8_T1_pre y \<Longrightarrow> U1FVars_2 t (pu p) \<subseteq> FFVars_T12 t \<union> PFVars_2 p \<union> avoiding_set2) \<Longrightarrow>
+  (\<And>t pu p. (t, pu) \<in> set9_T1_pre y \<union> set10_T1_pre y \<Longrightarrow> U2FVars_2 t (pu p) \<subseteq> FFVars_T22 t \<union> PFVars_2 p \<union> avoiding_set2) \<Longrightarrow>
+  U1FVars_2 (T1_ctor (map_T1_pre id id id id id id fst fst fst fst y)) (U1ctor y p) \<subseteq> FFVars_T12 (T1_ctor (map_T1_pre id id id id id id fst fst fst fst y)) \<union> PFVars_2 p \<union> avoiding_set2"
   (* model 2 axioms *)
 and U2map_id0: "U2map id id (t2::('var, 'tyvar, 'a, 'b) T2) = id"
-and U2map_comp0: "bij f1 \<Longrightarrow> |supp (f1::'var \<Rightarrow> 'var)| <o |UNIV::'var set| \<Longrightarrow> bij f2 \<Longrightarrow> |supp (g2::'tyvar \<Rightarrow> 'tyvar)| <o |UNIV::'tyvar set| \<Longrightarrow>
+and U2map_comp0: "bij f1 \<Longrightarrow> |supp (f1::'var \<Rightarrow> 'var)| <o |UNIV::'var set| \<Longrightarrow> bij f2 \<Longrightarrow> |supp (f2::'tyvar \<Rightarrow> 'tyvar)| <o |UNIV::'tyvar set| \<Longrightarrow>
   bij g1 \<Longrightarrow> |supp (g1::'var \<Rightarrow> 'var)| <o |UNIV::'var set| \<Longrightarrow> bij g2 \<Longrightarrow> |supp (g2::'tyvar \<Rightarrow> 'tyvar)| <o |UNIV::'tyvar set| \<Longrightarrow>
   U2map (g1 \<circ> f1) (g2 \<circ> f2) t2 = U2map g1 g2 t2 \<circ> U2map f1 f2 t2"
-and U2map_cong_id: "bij f1 \<Longrightarrow> |supp (f1::'var \<Rightarrow> 'var)| <o |UNIV::'var set| \<Longrightarrow> bij f2 \<Longrightarrow> |supp (g2::'tyvar \<Rightarrow> 'tyvar)| <o |UNIV::'tyvar set| \<Longrightarrow>
-  (\<And>a. a \<in> U2FVars_1 t2 u2 \<Longrightarrow> f1 a = a) \<Longrightarrow> (\<And>b. b \<in> U2FVars_2 t2 u2 \<Longrightarrow> f2 a = a) \<Longrightarrow>
+and U2map_cong_id: "bij f1 \<Longrightarrow> |supp (f1::'var \<Rightarrow> 'var)| <o |UNIV::'var set| \<Longrightarrow> bij f2 \<Longrightarrow> |supp (f2::'tyvar \<Rightarrow> 'tyvar)| <o |UNIV::'tyvar set| \<Longrightarrow>
+  (\<And>a. a \<in> U2FVars_1 t2 u2 \<Longrightarrow> f1 a = a) \<Longrightarrow> (\<And>a. a \<in> U2FVars_2 t2 u2 \<Longrightarrow> f2 a = a) \<Longrightarrow>
   U2map f1 f2 t2 u2 = u2"
-and U2FVars_Umap_1: "bij f1 \<Longrightarrow> |supp (f1::'var \<Rightarrow> 'var)| <o |UNIV::'var set| \<Longrightarrow> bij f2 \<Longrightarrow> |supp (g2::'tyvar \<Rightarrow> 'tyvar)| <o |UNIV::'tyvar set| \<Longrightarrow>
+and U2FVars_Umap_1: "bij f1 \<Longrightarrow> |supp (f1::'var \<Rightarrow> 'var)| <o |UNIV::'var set| \<Longrightarrow> bij f2 \<Longrightarrow> |supp (f2::'tyvar \<Rightarrow> 'tyvar)| <o |UNIV::'tyvar set| \<Longrightarrow>
   U2FVars_1 (rrename_T2 f1 f2 t2) (U2map f1 f2 t2 u2) = f1 ` U2FVars_1 t2 u2"
-and U2FVars_Umap_2: "bij f1 \<Longrightarrow> |supp (f1::'var \<Rightarrow> 'var)| <o |UNIV::'var set| \<Longrightarrow> bij f2 \<Longrightarrow> |supp (g2::'tyvar \<Rightarrow> 'tyvar)| <o |UNIV::'tyvar set| \<Longrightarrow>
+and U2FVars_Umap_2: "bij f1 \<Longrightarrow> |supp (f1::'var \<Rightarrow> 'var)| <o |UNIV::'var set| \<Longrightarrow> bij f2 \<Longrightarrow> |supp (f2::'tyvar \<Rightarrow> 'tyvar)| <o |UNIV::'tyvar set| \<Longrightarrow>
   U2FVars_2 (rrename_T2 f1 f2 t2) (U2map f1 f2 t2 u2) = f2 ` U2FVars_2 t2 u2"
-and U2map_Uctor: "bij f1 \<Longrightarrow> |supp (f1::'var \<Rightarrow> 'var)| <o |UNIV::'var set| \<Longrightarrow> bij f2 \<Longrightarrow> |supp (g2::'tyvar \<Rightarrow> 'tyvar)| <o |UNIV::'tyvar set| \<Longrightarrow>
+and U2map_Uctor: "bij f1 \<Longrightarrow> |supp (f1::'var \<Rightarrow> 'var)| <o |UNIV::'var set| \<Longrightarrow> bij f2 \<Longrightarrow> |supp (f2::'tyvar \<Rightarrow> 'tyvar)| <o |UNIV::'tyvar set| \<Longrightarrow>
   U2map f1 f2 (T2_ctor (map_T2_pre id id id id id id fst fst fst fst y2)) (U2ctor y2 p)
 = U2ctor (map_T2_pre f1 f2 id id f1 f2
-    (\<lambda>(t, pu). (rrename_T1 f1 f2 t, \<lambda>p. U1map f1 f2 t (pu p)))
-    (\<lambda>(t, pu). (rrename_T1 f1 f2 t, \<lambda>p. U1map f1 f2 t (pu p)))
-    (\<lambda>(t, pu). (rrename_T2 f1 f2 t, \<lambda>p. U2map f1 f2 t (pu p)))
-    (\<lambda>(t, pu). (rrename_T2 f1 f2 t, \<lambda>p. U2map f1 f2 t (pu p)))
+    (\<lambda>(t, pu). (rrename_T1 f1 f2 t, \<lambda>p. U1map f1 f2 t (pu (Pmap (inv f1) (inv f2) p))))
+    (\<lambda>(t, pu). (rrename_T1 f1 f2 t, \<lambda>p. U1map f1 f2 t (pu (Pmap (inv f1) (inv f2) p))))
+    (\<lambda>(t, pu). (rrename_T2 f1 f2 t, \<lambda>p. U2map f1 f2 t (pu (Pmap (inv f1) (inv f2) p))))
+    (\<lambda>(t, pu). (rrename_T2 f1 f2 t, \<lambda>p. U2map f1 f2 t (pu (Pmap (inv f1) (inv f2) p))))
  y2) (Pmap f1 f2 p)"
-and U2FVars_subset_1: "set5_T2_pre (y2::(_, _, 'a, 'b, _, _, _, _, _, _) T2_pre) \<inter> (PFVars_1 p \<union> avoiding_set2) = {} \<Longrightarrow>
-  (\<And>t pu p. (t, pu) \<in> set7_T2_pre y2 \<Longrightarrow> U1FVars_1 t (pu p) \<subseteq> FFVars_T11 t \<union> PFVars_1 p \<union> avoiding_set2) \<Longrightarrow>
-  (\<And>t pu p. (t, pu) \<in> set8_T2_pre y2 \<Longrightarrow> U1FVars_1 t (pu p) - set5_T2_pre y2 \<subseteq> FFVars_T11 t - set5_T2_pre y2 \<union> PFVars_1 p \<union> avoiding_set2) \<Longrightarrow>
-  (\<And>t pu p. (t, pu) \<in> set9_T2_pre y2 \<Longrightarrow> U2FVars_1 t (pu p) \<subseteq> FFVars_T21 t \<union> PFVars_1 p \<union> avoiding_set2) \<Longrightarrow>
-  (\<And>t pu p. (t, pu) \<in> set10_T2_pre y2 \<Longrightarrow> U2FVars_1 t (pu p) - set5_T2_pre y2 \<subseteq> FFVars_T21 t - set5_T2_pre y2 \<union> PFVars_1 p \<union> avoiding_set2) \<Longrightarrow>
-  U2FVars_1 (T2_ctor (map_T2_pre id id id id id id fst fst fst fst y2)) (U2ctor y2 p) \<subseteq> FFVars_T21 (T2_ctor (map_T2_pre id id id id id id fst fst fst fst y2)) \<union> set1_T2_pre y2 \<union> PFVars_1 p"
+and U2FVars_subset_1: "set5_T2_pre (y2::(_, _, 'a, 'b, _, _, _, _, _, _) T2_pre) \<inter> (PFVars_1 p \<union> avoiding_set1) = {} \<Longrightarrow>
+  (\<And>t pu p. (t, pu) \<in> set7_T2_pre y2 \<union> set8_T2_pre y2 \<Longrightarrow> U1FVars_1 t (pu p) \<subseteq> FFVars_T11 t \<union> PFVars_1 p \<union> avoiding_set1) \<Longrightarrow>
+  (\<And>t pu p. (t, pu) \<in> set9_T2_pre y2 \<union> set10_T2_pre y2 \<Longrightarrow> U2FVars_1 t (pu p) \<subseteq> FFVars_T21 t \<union> PFVars_1 p \<union> avoiding_set1) \<Longrightarrow>
+  U2FVars_1 (T2_ctor (map_T2_pre id id id id id id fst fst fst fst y2)) (U2ctor y2 p) \<subseteq> FFVars_T21 (T2_ctor (map_T2_pre id id id id id id fst fst fst fst y2)) \<union> PFVars_1 p \<union> avoiding_set1"
 and U2FVars_subset_2: "set6_T2_pre y2 \<inter> (PFVars_2 p \<union> avoiding_set2) = {} \<Longrightarrow>
-  (\<And>t pu p. (t, pu) \<in> set7_T2_pre y2 \<Longrightarrow> U1FVars_2 t (pu p) \<subseteq> FFVars_T12 t \<union> PFVars_2 p \<union> avoiding_set2) \<Longrightarrow>
-  (\<And>t pu p. (t, pu) \<in> set8_T2_pre y2 \<Longrightarrow> U1FVars_2 t (pu p) - set6_T2_pre y2 \<subseteq> FFVars_T12 t - set6_T2_pre y2 \<union> PFVars_2 p \<union> avoiding_set2) \<Longrightarrow>
-  (\<And>t pu p. (t, pu) \<in> set9_T2_pre y2 \<Longrightarrow> U2FVars_2 t (pu p) \<subseteq> FFVars_T22 t \<union> PFVars_2 p \<union> avoiding_set2) \<Longrightarrow>
-  (\<And>t pu p. (t, pu) \<in> set10_T2_pre y2 \<Longrightarrow> U2FVars_2 t (pu p) \<subseteq> FFVars_T22 t \<union> PFVars_2 p \<union> avoiding_set2) \<Longrightarrow>
-  U2FVars_2 (T2_ctor (map_T2_pre id id id id id id fst fst fst fst y2)) (U2ctor y2 p) \<subseteq> FFVars_T22 (T2_ctor (map_T2_pre id id id id id id fst fst fst fst y2)) \<union> set2_T2_pre y2 \<union> PFVars_2 p"
+  (\<And>t pu p. (t, pu) \<in> set7_T2_pre y2 \<union> set8_T2_pre y2 \<Longrightarrow> U1FVars_2 t (pu p) \<subseteq> FFVars_T12 t \<union> PFVars_2 p \<union> avoiding_set2) \<Longrightarrow>
+  (\<And>t pu p. (t, pu) \<in> set9_T2_pre y2 \<union> set10_T2_pre y2 \<Longrightarrow> U2FVars_2 t (pu p) \<subseteq> FFVars_T22 t \<union> PFVars_2 p \<union> avoiding_set2) \<Longrightarrow>
+  U2FVars_2 (T2_ctor (map_T2_pre id id id id id id fst fst fst fst y2)) (U2ctor y2 p) \<subseteq> FFVars_T22 (T2_ctor (map_T2_pre id id id id id id fst fst fst fst y2)) \<union> PFVars_2 p \<union> avoiding_set2"
 print_theorems
+
+lemmas U1FVars_subsets = U1FVars_subset_1 U1FVars_subset_2
+lemmas U2FVars_subsets = U2FVars_subset_1 U2FVars_subset_2
+
+(**********************************************************************)
+(*                            DEFINITIONS                             *)
+(**********************************************************************)
 
 type_synonym ('var, 'tyvar, 'a, 'b) pre_T1 = "('var, 'tyvar, 'a, 'b, 'var, 'tyvar,
   ('var, 'tyvar, 'a, 'b) raw_T1, ('var, 'tyvar, 'a, 'b) raw_T1,
@@ -140,6 +139,13 @@ definition suitable21 :: "(('var::{var_T1_pre,var_T2_pre}, 'tyvar::{var_T1_pre,v
   "suitable21 \<equiv> \<lambda>pick. \<forall>x p. bij (pick x p) \<and> |supp (pick x p)| <o |UNIV::'var set|
   \<and> imsupp (pick x p) \<inter> ((FVars_T21 (raw_T2_ctor x) \<union> PFVars_1 p \<union> avoiding_set1) - set5_T2_pre x) = {}
   \<and> (pick x p) ` set5_T2_pre x \<inter> (FVars_T21 (raw_T2_ctor x) \<union> PFVars_1 p \<union> avoiding_set1) = {}"
+
+definition suitable22 :: "(('var::{var_T1_pre,var_T2_pre}, 'tyvar::{var_T1_pre,var_T2_pre}, 'a::{var_T1_pre,var_T2_pre}, 'b) pre_T2 \<Rightarrow> ('var, 'tyvar) P \<Rightarrow> 'tyvar \<Rightarrow> 'tyvar) \<Rightarrow> bool" where
+  "suitable22 \<equiv> \<lambda>pick. \<forall>x p. bij (pick x p) \<and> |supp (pick x p)| <o |UNIV::'tyvar set|
+  \<and> imsupp (pick x p) \<inter> ((FVars_T22 (raw_T2_ctor x) \<union> PFVars_2 p \<union> avoiding_set2) - set6_T2_pre x) = {}
+  \<and> (pick x p) ` set6_T2_pre x \<inter> (FVars_T22 (raw_T2_ctor x) \<union> PFVars_2 p \<union> avoiding_set2) = {}"
+
+lemmas suitable_defs = suitable11_def suitable12_def suitable21_def suitable22_def
 
 abbreviation "abs_T1 \<equiv> quot_type.abs alpha_T1 Abs_T1"
 abbreviation "abs_T2 \<equiv> quot_type.abs alpha_T2 Abs_T2"
@@ -176,7 +182,8 @@ lemma suitable_bij:
   "suitable11 pick1 \<Longrightarrow> bij (pick1 x p)"
   "suitable12 pick2 \<Longrightarrow> bij (pick2 x p)"
   "suitable21 pick3 \<Longrightarrow> bij (pick3 x' p)"
-    apply (unfold suitable11_def suitable12_def suitable21_def)
+  "suitable22 pick4 \<Longrightarrow> bij (pick4 x' p)"
+    apply (unfold suitable_defs)
     apply ((erule allE conjE)+, assumption)+
   done
 
@@ -184,26 +191,27 @@ lemma suitable_supp_bound:
   "suitable11 pick1 \<Longrightarrow> |supp (pick1 x (p::('var::{var_T1_pre,var_T2_pre}, 'tyvar::{var_T1_pre,var_T2_pre}) P))| <o |UNIV::'var set|"
   "suitable12 pick2 \<Longrightarrow> |supp (pick2 x p)| <o |UNIV::'tyvar set|"
   "suitable21 pick3 \<Longrightarrow> |supp (pick3 x' p)| <o |UNIV::'var set|"
-    apply (unfold suitable11_def suitable12_def suitable21_def)
+  "suitable22 pick4 \<Longrightarrow> |supp (pick4 x' p)| <o |UNIV::'tyvar set|"
+    apply (unfold suitable_defs)
     apply ((erule allE conjE)+, assumption)+
   done
 
-function f_T1 :: "_ \<Rightarrow> _ \<Rightarrow> _ \<Rightarrow> _ \<Rightarrow> _ \<Rightarrow> ('var::{var_T1_pre,var_T2_pre}, 'tyvar::{var_T1_pre,var_T2_pre}, 'a::{var_T1_pre,var_T2_pre}, 'b) U1"
-  and f_T2 :: "_ \<Rightarrow> _ \<Rightarrow> _ \<Rightarrow> _ \<Rightarrow> _ \<Rightarrow> ('var, 'tyvar, 'a, 'b) U2" where
-  "f_T1 pick1 pick2 pick3 (raw_T1_ctor x) p = (if suitable11 pick1 \<and> suitable12 pick2 \<and> suitable21 pick3 then
+function f_T1 :: "_ \<Rightarrow> _ \<Rightarrow> _ \<Rightarrow> _ \<Rightarrow> _ \<Rightarrow> _ \<Rightarrow> ('var::{var_T1_pre,var_T2_pre}, 'tyvar::{var_T1_pre,var_T2_pre}, 'a::{var_T1_pre,var_T2_pre}, 'b) U1"
+  and f_T2 :: "_ \<Rightarrow> _ \<Rightarrow> _ \<Rightarrow> _ \<Rightarrow> _ \<Rightarrow> _ \<Rightarrow> ('var, 'tyvar, 'a, 'b) U2" where
+  "f_T1 pick1 pick2 pick3 pick4 (raw_T1_ctor x) p = (if suitable11 pick1 \<and> suitable12 pick2 \<and> suitable21 pick3 \<and> suitable22 pick4 then
   U1ctor' (map_T1_pre id id id id id id
-    (\<lambda>t. (t, f_T1 pick1 pick2 pick3 t)) (\<lambda>t. (t, f_T1 pick1 pick2 pick3 t))
-    (\<lambda>t. (t, f_T2 pick1 pick2 pick3 t)) (\<lambda>t. (t, f_T2 pick1 pick2 pick3 t)) (
+    (\<lambda>t. (t, f_T1 pick1 pick2 pick3 pick4 t)) (\<lambda>t. (t, f_T1 pick1 pick2 pick3 pick4 t))
+    (\<lambda>t. (t, f_T2 pick1 pick2 pick3 pick4 t)) (\<lambda>t. (t, f_T2 pick1 pick2 pick3 pick4 t)) (
   map_T1_pre id id id id (pick1 x p) (pick2 x p) id
     (rename_T1 (pick1 x p) (pick2 x p)) id (rename_T2 (pick1 x p) (pick2 x p)) x
   )) p
 else undefined)"
-| "f_T2 pick1 pick2 pick3 (raw_T2_ctor x) p = (if suitable11 pick1 \<and> suitable12 pick2 \<and> suitable21 pick3 then
+| "f_T2 pick1 pick2 pick3 pick4 (raw_T2_ctor x) p = (if suitable11 pick1 \<and> suitable12 pick2 \<and> suitable21 pick3 \<and> suitable22 pick4 then
   U2ctor' (map_T2_pre id id id id id id
-    (\<lambda>t. (t, f_T1 pick1 pick2 pick3 t)) (\<lambda>t. (t, f_T1 pick1 pick2 pick3 t))
-    (\<lambda>t. (t, f_T2 pick1 pick2 pick3 t)) (\<lambda>t. (t, f_T2 pick1 pick2 pick3 t)) (
-  map_T2_pre id id id id (pick3 x p) id id
-    (rename_T1 (pick3 x p) id) id (rename_T2 (pick3 x p) id) x
+    (\<lambda>t. (t, f_T1 pick1 pick2 pick3 pick4 t)) (\<lambda>t. (t, f_T1 pick1 pick2 pick3 pick4 t))
+    (\<lambda>t. (t, f_T2 pick1 pick2 pick3 pick4 t)) (\<lambda>t. (t, f_T2 pick1 pick2 pick3 pick4 t)) (
+  map_T2_pre id id id id (pick3 x p) (pick4 x p) id
+    (rename_T1 (pick3 x p) (pick4 x p)) id (rename_T2 (pick3 x p) (pick4 x p)) x
   )) p
 else undefined)"
      apply pat_completeness
@@ -212,7 +220,7 @@ termination
   apply (relation "inv_image {(x, y). case x of
     Inl t1 \<Rightarrow> (case y of Inl t1' \<Rightarrow> subshape_T1_T1 t1 t1' | Inr t2 \<Rightarrow> subshape_T1_T2 t1 t2)
   | Inr t2 \<Rightarrow> (case y of Inl t1 \<Rightarrow> subshape_T2_T1 t2 t1 | Inr t2' \<Rightarrow> subshape_T2_T2 t2 t2')
- } (map_sum (fst \<circ> snd \<circ> snd \<circ> snd) (fst \<circ> snd \<circ> snd \<circ> snd))")
+ } (map_sum (fst \<circ> snd \<circ> snd \<circ> snd \<circ> snd) (fst \<circ> snd \<circ> snd \<circ> snd \<circ> snd))")
           apply (rule wf_inv_image)
           apply (rule T1.wf_subshape)
 
@@ -302,13 +310,13 @@ termination
   done
 print_theorems
 
-lemma f_T1_simp: "suitable11 pick1 \<Longrightarrow> suitable12 pick2 \<Longrightarrow> suitable21 pick3 \<Longrightarrow>
-  f_T1 pick1 pick2 pick3 (raw_T1_ctor x) p =
+lemma f_T1_simp: "suitable11 pick1 \<Longrightarrow> suitable12 pick2 \<Longrightarrow> suitable21 pick3 \<Longrightarrow> suitable22 pick4 \<Longrightarrow>
+  f_T1 pick1 pick2 pick3 pick4 (raw_T1_ctor x) p =
     U1ctor' (map_T1_pre id id id id (pick1 x p) (pick2 x p)
-      (\<lambda>t. (t, f_T1 pick1 pick2 pick3 t))
-      (\<lambda>t. (rename_T1 (pick1 x p) (pick2 x p) t, f_T1 pick1 pick2 pick3 (rename_T1 (pick1 x p) (pick2 x p) t)))
-      (\<lambda>t. (t, f_T2 pick1 pick2 pick3 t))
-      (\<lambda>t. (rename_T2 (pick1 x p) (pick2 x p) t, f_T2 pick1 pick2 pick3 (rename_T2 (pick1 x p) (pick2 x p) t)))
+      (\<lambda>t. (t, f_T1 pick1 pick2 pick3 pick4 t))
+      (\<lambda>t. (rename_T1 (pick1 x p) (pick2 x p) t, f_T1 pick1 pick2 pick3 pick4 (rename_T1 (pick1 x p) (pick2 x p) t)))
+      (\<lambda>t. (t, f_T2 pick1 pick2 pick3 pick4 t))
+      (\<lambda>t. (rename_T2 (pick1 x p) (pick2 x p) t, f_T2 pick1 pick2 pick3 pick4 (rename_T2 (pick1 x p) (pick2 x p) t)))
      x) p"
   apply (unfold f_T1.simps)
   apply (subst if_P)
@@ -321,13 +329,13 @@ lemma f_T1_simp: "suitable11 pick1 \<Longrightarrow> suitable12 pick2 \<Longrigh
   apply (unfold comp_def)
   apply (rule refl)
   done
-lemma f_T2_simp: "suitable11 pick1 \<Longrightarrow> suitable12 pick2 \<Longrightarrow> suitable21 pick3 \<Longrightarrow>
-  f_T2 pick1 pick2 pick3 (raw_T2_ctor x) p =
-    U2ctor' (map_T2_pre id id id id (pick3 x p) id
-      (\<lambda>t. (t, f_T1 pick1 pick2 pick3 t))
-      (\<lambda>t. (rename_T1 (pick3 x p) id t, f_T1 pick1 pick2 pick3 (rename_T1 (pick3 x p) id t)))
-      (\<lambda>t. (t, f_T2 pick1 pick2 pick3 t))
-      (\<lambda>t. (rename_T2 (pick3 x p) id t, f_T2 pick1 pick2 pick3 (rename_T2 (pick3 x p) id t)))
+lemma f_T2_simp: "suitable11 pick1 \<Longrightarrow> suitable12 pick2 \<Longrightarrow> suitable21 pick3 \<Longrightarrow> suitable22 pick4 \<Longrightarrow>
+  f_T2 pick1 pick2 pick3 pick4 (raw_T2_ctor x) p =
+    U2ctor' (map_T2_pre id id id id (pick3 x p) (pick4 x p)
+      (\<lambda>t. (t, f_T1 pick1 pick2 pick3 pick4 t))
+      (\<lambda>t. (rename_T1 (pick3 x p) (pick4 x p) t, f_T1 pick1 pick2 pick3 pick4 (rename_T1 (pick3 x p) (pick4 x p) t)))
+      (\<lambda>t. (t, f_T2 pick1 pick2 pick3 pick4 t))
+      (\<lambda>t. (rename_T2 (pick3 x p) (pick4 x p) t, f_T2 pick1 pick2 pick3 pick4 (rename_T2 (pick3 x p) (pick4 x p) t)))
      x) p"
   apply (unfold f_T2.simps)
   apply (subst if_P)
@@ -344,14 +352,527 @@ lemma f_T2_simp: "suitable11 pick1 \<Longrightarrow> suitable12 pick2 \<Longrigh
 definition "pick1_0 \<equiv> SOME pick. suitable11 pick"
 definition "pick2_0 \<equiv> SOME pick. suitable12 pick"
 definition "pick3_0 \<equiv> SOME pick. suitable21 pick"
+definition "pick4_0 \<equiv> SOME pick. suitable22 pick"
 
-definition "f0_T1 \<equiv> f_T1 pick1_0 pick2_0 pick3_0"
-definition "f0_T2 \<equiv> f_T2 pick1_0 pick2_0 pick3_0"
+definition "f0_T1 \<equiv> f_T1 pick1_0 pick2_0 pick3_0 pick4_0"
+definition "f0_T2 \<equiv> f_T2 pick1_0 pick2_0 pick3_0 pick4_0"
 
 abbreviation "rep_T1 \<equiv> quot_type.rep Rep_T1"
 abbreviation "rep_T2 \<equiv> quot_type.rep Rep_T2"
 
 definition "ff0_T1 t \<equiv> f0_T1 (rep_T1 t)"
 definition "ff0_T2 t \<equiv> f0_T2 (rep_T2 t)"
+
+definition noclash_T1 :: "('var::{var_T1_pre,var_T2_pre}, 'tyvar::{var_T1_pre,var_T2_pre}, 'a::{var_T1_pre,var_T2_pre}, 'b) pre_T1 \<Rightarrow> bool" where
+  "noclash_T1 x \<equiv> (
+    (set5_T1_pre x \<inter> (set1_T1_pre x \<union> \<Union>(FVars_T11 ` set7_T1_pre x) \<union> \<Union>(FVars_T21 ` set9_T1_pre x)) = {})
+    \<and> (set6_T1_pre x \<inter> (set2_T1_pre x \<union> \<Union>(FVars_T12 ` set7_T1_pre x) \<union> \<Union>(FVars_T22 ` set9_T1_pre x) \<union> \<Union>(FVars_T22 ` set10_T1_pre x)) = {})
+  )"
+definition noclash_T2 :: "('var::{var_T1_pre,var_T2_pre}, 'tyvar::{var_T1_pre,var_T2_pre}, 'a::{var_T1_pre,var_T2_pre}, 'b) pre_T2 \<Rightarrow> bool" where
+  "noclash_T2 x \<equiv> (
+    (set5_T2_pre x \<inter> (set1_T2_pre x \<union> \<Union>(FVars_T11 ` set7_T2_pre x) \<union> \<Union>(FVars_T21 ` set9_T2_pre x)) = {})
+    \<and> (set6_T2_pre x \<inter> (set2_T2_pre x \<union> \<Union>(FVars_T12 ` set7_T2_pre x) \<union> \<Union>(FVars_T22 ` set9_T2_pre x) \<union> \<Union>(FVars_T22 ` set10_T2_pre x)) = {})
+  )"
+
+type_synonym ('var, 'tyvar, 'a, 'b) pre_TT1 = "('var, 'tyvar, 'a, 'b, 'var, 'tyvar,
+  ('var, 'tyvar, 'a, 'b) T1, ('var, 'tyvar, 'a, 'b) T1,
+  ('var, 'tyvar, 'a, 'b) T2, ('var, 'tyvar, 'a, 'b) T2
+) T1_pre"
+type_synonym ('var, 'tyvar, 'a, 'b) pre_TT2 = "('var, 'tyvar, 'a, 'b, 'var, 'tyvar,
+  ('var, 'tyvar, 'a, 'b) T1, ('var, 'tyvar, 'a, 'b) T1,
+  ('var, 'tyvar, 'a, 'b) T2, ('var, 'tyvar, 'a, 'b) T2
+) T2_pre"
+
+definition nnoclash_T1 :: "('var::{var_T1_pre,var_T2_pre}, 'tyvar::{var_T1_pre,var_T2_pre}, 'a::{var_T1_pre,var_T2_pre}, 'b) pre_TT1 \<Rightarrow> bool" where
+  "nnoclash_T1 x \<equiv> (
+    (set5_T1_pre x \<inter> (set1_T1_pre x \<union> \<Union>(FFVars_T11 ` set7_T1_pre x) \<union> \<Union>(FFVars_T21 ` set9_T1_pre x)) = {})
+    \<and> (set6_T1_pre x \<inter> (set2_T1_pre x \<union> \<Union>(FFVars_T12 ` set7_T1_pre x) \<union> \<Union>(FFVars_T22 ` set9_T1_pre x) \<union> \<Union>(FFVars_T22 ` set10_T1_pre x)) = {})
+  )"
+definition nnoclash_T2 :: "('var::{var_T1_pre,var_T2_pre}, 'tyvar::{var_T1_pre,var_T2_pre}, 'a::{var_T1_pre,var_T2_pre}, 'b) pre_TT2 \<Rightarrow> bool" where
+  "nnoclash_T2 x \<equiv> (
+    (set5_T2_pre x \<inter> (set1_T2_pre x \<union> \<Union>(FFVars_T11 ` set7_T2_pre x) \<union> \<Union>(FFVars_T21 ` set9_T2_pre x)) = {})
+    \<and> (set6_T2_pre x \<inter> (set2_T2_pre x \<union> \<Union>(FFVars_T12 ` set7_T2_pre x) \<union> \<Union>(FFVars_T22 ` set9_T2_pre x) \<union> \<Union>(FFVars_T22 ` set10_T2_pre x)) = {})
+  )"
+
+(* TODO: XXl and XXr *)
+
+(**********************************************************************)
+(*                               PROOFS                               *)
+(**********************************************************************)
+
+lemma pick_id_ons:
+  "suitable11 pick1 \<Longrightarrow> id_on (\<Union>(FVars_T11 ` set8_T1_pre x) - set5_T1_pre x) (pick1 x p)"
+  "suitable11 pick1 \<Longrightarrow> id_on (\<Union>(FVars_T21 ` set10_T1_pre x) - set5_T1_pre x) (pick1 x p)"
+  "suitable12 pick2 \<Longrightarrow> id_on (\<Union>(FVars_T12 ` set8_T1_pre x) - set6_T1_pre x) (pick2 x p)"
+  "suitable21 pick3 \<Longrightarrow> id_on (\<Union>(FVars_T11 ` set8_T2_pre y) - set5_T2_pre y) (pick3 y p)"
+  "suitable21 pick3 \<Longrightarrow> id_on (\<Union>(FVars_T21 ` set10_T2_pre y) - set5_T2_pre y) (pick3 y p)"
+  "suitable22 pick4 \<Longrightarrow> id_on (\<Union>(FVars_T12 ` set8_T2_pre y) - set6_T2_pre y) (pick4 y p)"
+    apply (unfold suitable_defs Int_Un_distrib Un_empty Un_Diff Diff_idemp T1.FVars_ctors)
+
+  (* ALLGOALS *)
+    apply (erule allE conjE)+
+    apply (rule imsupp_id_on)
+  apply assumption
+  (* copied from above*)
+  apply (erule allE conjE)+
+    apply (rule imsupp_id_on)
+   apply assumption
+   apply (erule allE conjE)+
+    apply (rule imsupp_id_on)
+  apply assumption
+   apply (erule allE conjE)+
+    apply (rule imsupp_id_on)
+   apply assumption
+   apply (erule allE conjE)+
+    apply (rule imsupp_id_on)
+   apply assumption
+   apply (erule allE conjE)+
+    apply (rule imsupp_id_on)
+  apply assumption
+  done
+
+lemma pick_id_on_images:
+  fixes f1::"'var::{var_T1_pre,var_T2_pre} \<Rightarrow> 'var" and f2::"'tyvar::{var_T1_pre,var_T2_pre} \<Rightarrow> 'tyvar"
+  assumes "bij f1" "|supp f1| <o |UNIV::'var set|" "bij f2" "|supp f2| <o |UNIV::'tyvar set|"
+  shows
+  "suitable11 pick1 \<Longrightarrow> id_on (f1 ` (\<Union>(FVars_T11 ` set8_T1_pre x) - set5_T1_pre x)) (pick1 (map_T1_pre f1 f2 id id f1 f2 (rename_T1 f1 f2) (rename_T1 f1 f2) (rename_T2 f1 f2) (rename_T2 f1 f2) x) p)"
+  "suitable11 pick1 \<Longrightarrow> id_on (f1 ` (\<Union>(FVars_T21 ` set10_T1_pre x) - set5_T1_pre x)) (pick1 (map_T1_pre f1 f2 id id f1 f2 (rename_T1 f1 f2) (rename_T1 f1 f2) (rename_T2 f1 f2) (rename_T2 f1 f2) x) p)"
+  "suitable12 pick2 \<Longrightarrow> id_on (f2 ` (\<Union>(FVars_T12 ` set8_T1_pre x) - set6_T1_pre x)) (pick2 (map_T1_pre f1 f2 id id f1 f2 (rename_T1 f1 f2) (rename_T1 f1 f2) (rename_T2 f1 f2) (rename_T2 f1 f2) x) p)"
+  "suitable21 pick3 \<Longrightarrow> id_on (f1 ` (\<Union>(FVars_T11 ` set8_T2_pre y) - set5_T2_pre y)) (pick3 (map_T2_pre f1 f2 id id f1 f2 (rename_T1 f1 f2) (rename_T1 f1 f2) (rename_T2 f1 f2) (rename_T2 f1 f2) y) p)"
+  "suitable21 pick3 \<Longrightarrow> id_on (f1 ` (\<Union>(FVars_T21 ` set10_T2_pre y) - set5_T2_pre y)) (pick3 (map_T2_pre f1 f2 id id f1 f2 (rename_T1 f1 f2) (rename_T1 f1 f2) (rename_T2 f1 f2) (rename_T2 f1 f2) y) p)"
+  "suitable22 pick4 \<Longrightarrow> id_on (f2 ` (\<Union>(FVars_T12 ` set8_T2_pre y) - set6_T2_pre y)) (pick4 (map_T2_pre f1 f2 id id f1 f2 (rename_T1 f1 f2) (rename_T1 f1 f2) (rename_T2 f1 f2) (rename_T2 f1 f2) y) p)"
+       apply -
+  (* EVERY' (map ... pick_id_ons) *)
+       apply (rule iffD2[OF arg_cong2[OF _ refl, of _ _ id_on], rotated])
+        apply (erule pick_id_ons(1))
+       apply (subst T1_pre.set_map T2_pre.set_map T1.FVars_renames image_set_diff[OF bij_is_inj] comp_def image_comp image_UN,
+          ((rule supp_id_bound bij_id assms)+)?
+       )+
+       apply (rule refl)
+  (* copied from above (incremented index) *)
+       apply (rule iffD2[OF arg_cong2[OF _ refl, of _ _ id_on], rotated])
+        apply (erule pick_id_ons(2))
+       apply (subst T1_pre.set_map T2_pre.set_map T1.FVars_renames image_set_diff[OF bij_is_inj] comp_def image_comp image_UN,
+          ((rule supp_id_bound bij_id assms)+)?
+       )+
+      apply (rule refl)
+apply (rule iffD2[OF arg_cong2[OF _ refl, of _ _ id_on], rotated])
+        apply (erule pick_id_ons(3))
+       apply (subst T1_pre.set_map T2_pre.set_map T1.FVars_renames image_set_diff[OF bij_is_inj] comp_def image_comp image_UN,
+          ((rule supp_id_bound bij_id assms)+)?
+       )+
+  apply (rule refl)
+apply (rule iffD2[OF arg_cong2[OF _ refl, of _ _ id_on], rotated])
+        apply (erule pick_id_ons(4))
+       apply (subst T1_pre.set_map T2_pre.set_map T1.FVars_renames image_set_diff[OF bij_is_inj] comp_def image_comp image_UN,
+          ((rule supp_id_bound bij_id assms)+)?
+       )+
+  apply (rule refl)
+apply (rule iffD2[OF arg_cong2[OF _ refl, of _ _ id_on], rotated])
+        apply (erule pick_id_ons(5))
+       apply (subst T1_pre.set_map T2_pre.set_map T1.FVars_renames image_set_diff[OF bij_is_inj] comp_def image_comp image_UN,
+          ((rule supp_id_bound bij_id assms)+)?
+       )+
+  apply (rule refl)
+apply (rule iffD2[OF arg_cong2[OF _ refl, of _ _ id_on], rotated])
+        apply (erule pick_id_ons(6))
+       apply (subst T1_pre.set_map T2_pre.set_map T1.FVars_renames image_set_diff[OF bij_is_inj] comp_def image_comp image_UN,
+          ((rule supp_id_bound bij_id assms)+)?
+       )+
+  apply (rule refl)
+  done
+
+(* lower axioms to raw type *)
+lemma U1map'_U1ctor': "bij f1 \<Longrightarrow> |supp (f1::'var::{var_T1_pre,var_T2_pre} \<Rightarrow> 'var)| <o |UNIV::'var set| \<Longrightarrow> bij f2 \<Longrightarrow> |supp (f2::'tyvar::{var_T1_pre,var_T2_pre} \<Rightarrow> 'tyvar)| <o |UNIV::'tyvar set| \<Longrightarrow>
+  U1map' f1 f2 (raw_T1_ctor (map_T1_pre id id id id id id fst fst fst fst y)) (U1ctor' y p)
+= U1ctor' (map_T1_pre f1 f2 id id f1 f2
+    (\<lambda>(t, pu). (rename_T1 f1 f2 t, PU1map' f1 f2 t pu))
+    (\<lambda>(t, pu). (rename_T1 f1 f2 t, PU1map' f1 f2 t pu))
+    (\<lambda>(t, pu). (rename_T2 f1 f2 t, PU2map' f1 f2 t pu))
+    (\<lambda>(t, pu). (rename_T2 f1 f2 t, PU2map' f1 f2 t pu))
+ y) (Pmap f1 f2 p)"
+  apply (unfold U1map'_def U2map'_def U1ctor'_def U2ctor'_def PU1map'_def PU2map'_def T1.TT_abs_ctors)
+  apply (subst T1_pre.map_comp T2_pre.map_comp, (rule supp_id_bound bij_id)+)
+  apply (unfold fst_comp_map_prod)
+  apply (subst T1_pre.map_comp[symmetric] T2_pre.map_comp[symmetric], (rule supp_id_bound bij_id)+)
+  apply (rule trans)
+   apply (rule U1map_Uctor U2map_Uctor)
+      apply assumption+
+  apply (rule arg_cong2[OF _ refl, of _ _ U1ctor] arg_cong2[OF _ refl, of _ _ U2ctor])
+  apply (rule trans)
+   apply (rule T1_pre.map_comp T2_pre.map_comp)
+                apply (rule supp_id_bound bij_id | assumption)+
+  apply (rule sym)
+  apply (rule trans)
+   apply (rule T1_pre.map_comp T2_pre.map_comp)
+                apply (rule supp_id_bound bij_id | assumption)+
+  apply (unfold id_o o_id)
+  apply (rule T1_pre.map_cong T2_pre.map_cong)
+                      apply (rule supp_id_bound bij_id | assumption)+
+     apply (unfold comp_def case_prod_map_prod split_beta fst_map_prod snd_map_prod map_prod_simp id_def)
+  (* ALLGOALS (refl ORELSE ...) *) apply (rule refl)+
+     apply (rule iffD2[OF prod.inject])
+     apply (rule conjI)
+      apply (unfold rrename_T1_def rrename_T2_def)[1]
+      apply (rule T1.TT_Quotient_total_abs_eq_iffs[THEN iffD2])
+      apply (rule T1.alpha_bij_eqs[THEN iffD2])
+          apply (rule supp_id_bound bij_id | assumption)+
+      apply (rule T1.TT_alpha_quotient_syms)
+     apply (rule refl)
+  (* copied from above *)
+apply (rule iffD2[OF prod.inject])
+     apply (rule conjI)
+      apply (unfold rrename_T1_def rrename_T2_def)[1]
+      apply (rule T1.TT_Quotient_total_abs_eq_iffs[THEN iffD2])
+      apply (rule T1.alpha_bij_eqs[THEN iffD2])
+          apply (rule supp_id_bound bij_id | assumption)+
+      apply (rule T1.TT_alpha_quotient_syms)
+    apply (rule refl)
+apply (rule iffD2[OF prod.inject])
+     apply (rule conjI)
+      apply (unfold rrename_T1_def rrename_T2_def)[1]
+      apply (rule T1.TT_Quotient_total_abs_eq_iffs[THEN iffD2])
+      apply (rule T1.alpha_bij_eqs[THEN iffD2])
+          apply (rule supp_id_bound bij_id | assumption)+
+      apply (rule T1.TT_alpha_quotient_syms)
+   apply (rule refl)
+apply (rule iffD2[OF prod.inject])
+     apply (rule conjI)
+      apply (unfold rrename_T1_def rrename_T2_def)[1]
+      apply (rule T1.TT_Quotient_total_abs_eq_iffs[THEN iffD2])
+      apply (rule T1.alpha_bij_eqs[THEN iffD2])
+          apply (rule supp_id_bound bij_id | assumption)+
+      apply (rule T1.TT_alpha_quotient_syms)
+  apply (rule refl)
+  done
+lemma U2map'_Uctor': "bij f1 \<Longrightarrow> |supp (f1::'var::{var_T1_pre,var_T2_pre} \<Rightarrow> 'var)| <o |UNIV::'var set| \<Longrightarrow> bij f2 \<Longrightarrow> |supp (f2::'tyvar::{var_T1_pre,var_T2_pre} \<Rightarrow> 'tyvar)| <o |UNIV::'tyvar set| \<Longrightarrow>
+  U2map' f1 f2 (raw_T2_ctor (map_T2_pre id id id id id id fst fst fst fst y2)) (U2ctor' y2 p)
+= U2ctor' (map_T2_pre f1 f2 id id f1 f2
+    (\<lambda>(t, pu). (rename_T1 f1 f2 t, PU1map' f1 f2 t pu))
+    (\<lambda>(t, pu). (rename_T1 f1 f2 t, PU1map' f1 f2 t pu))
+    (\<lambda>(t, pu). (rename_T2 f1 f2 t, PU2map' f1 f2 t pu))
+    (\<lambda>(t, pu). (rename_T2 f1 f2 t, PU2map' f1 f2 t pu))
+ y2) (Pmap f1 f2 p)"
+  (* same tactic as above *)
+  apply (unfold U1map'_def U2map'_def U1ctor'_def U2ctor'_def PU1map'_def PU2map'_def T1.TT_abs_ctors)
+  apply (subst T1_pre.map_comp T2_pre.map_comp, (rule supp_id_bound bij_id)+)
+  apply (unfold fst_comp_map_prod)
+  apply (subst T1_pre.map_comp[symmetric] T2_pre.map_comp[symmetric], (rule supp_id_bound bij_id)+)
+  apply (rule trans)
+   apply (rule U1map_Uctor U2map_Uctor)
+      apply assumption+
+  apply (rule arg_cong2[OF _ refl, of _ _ U1ctor] arg_cong2[OF _ refl, of _ _ U2ctor])
+  apply (rule trans)
+   apply (rule T1_pre.map_comp T2_pre.map_comp)
+                apply (rule supp_id_bound bij_id | assumption)+
+  apply (rule sym)
+  apply (rule trans)
+   apply (rule T1_pre.map_comp T2_pre.map_comp)
+                apply (rule supp_id_bound bij_id | assumption)+
+  apply (unfold id_o o_id)
+  apply (rule T1_pre.map_cong T2_pre.map_cong)
+                      apply (rule supp_id_bound bij_id | assumption)+
+     apply (unfold comp_def case_prod_map_prod split_beta fst_map_prod snd_map_prod map_prod_simp id_def)
+  apply (rule refl)+
+     apply (rule iffD2[OF prod.inject])
+     apply (rule conjI)
+      apply (unfold rrename_T1_def rrename_T2_def)[1]
+      apply (rule T1.TT_Quotient_total_abs_eq_iffs[THEN iffD2])
+      apply (rule T1.alpha_bij_eqs[THEN iffD2])
+          apply (rule supp_id_bound bij_id | assumption)+
+      apply (rule T1.TT_alpha_quotient_syms)
+     apply (rule refl)
+apply (rule iffD2[OF prod.inject])
+     apply (rule conjI)
+      apply (unfold rrename_T1_def rrename_T2_def)[1]
+      apply (rule T1.TT_Quotient_total_abs_eq_iffs[THEN iffD2])
+      apply (rule T1.alpha_bij_eqs[THEN iffD2])
+          apply (rule supp_id_bound bij_id | assumption)+
+      apply (rule T1.TT_alpha_quotient_syms)
+    apply (rule refl)
+apply (rule iffD2[OF prod.inject])
+     apply (rule conjI)
+      apply (unfold rrename_T1_def rrename_T2_def)[1]
+      apply (rule T1.TT_Quotient_total_abs_eq_iffs[THEN iffD2])
+      apply (rule T1.alpha_bij_eqs[THEN iffD2])
+          apply (rule supp_id_bound bij_id | assumption)+
+      apply (rule T1.TT_alpha_quotient_syms)
+   apply (rule refl)
+apply (rule iffD2[OF prod.inject])
+     apply (rule conjI)
+      apply (unfold rrename_T1_def rrename_T2_def)[1]
+      apply (rule T1.TT_Quotient_total_abs_eq_iffs[THEN iffD2])
+      apply (rule T1.alpha_bij_eqs[THEN iffD2])
+          apply (rule supp_id_bound bij_id | assumption)+
+      apply (rule T1.TT_alpha_quotient_syms)
+  apply (rule refl)
+  done
+
+lemmas FVars_def2s = T1.alpha_FVarss(1)[OF T1.TT_alpha_quotient_syms(1),
+  unfolded fun_cong[OF meta_eq_to_obj_eq[OF FFVars_T11_def], symmetric]
+] T1.alpha_FVarss(2)[OF T1.TT_alpha_quotient_syms(2),
+  unfolded fun_cong[OF meta_eq_to_obj_eq[OF FFVars_T21_def], symmetric]
+] T1.alpha_FVarss(3)[OF T1.TT_alpha_quotient_syms(1),
+  unfolded fun_cong[OF meta_eq_to_obj_eq[OF FFVars_T12_def], symmetric]
+] T1.alpha_FVarss(4)[OF T1.TT_alpha_quotient_syms(2),
+  unfolded fun_cong[OF meta_eq_to_obj_eq[OF FFVars_T22_def], symmetric]
+]
+
+lemma U1FVars'_subsets: "set5_T1_pre (y::(_, _, 'a::{var_T1_pre,var_T2_pre}, 'b, _, _, _, _, _, _) T1_pre) \<inter> (PFVars_1 p \<union> avoiding_set1) = {} \<Longrightarrow>
+  (\<And>t pu p. (t, pu) \<in> set7_T1_pre y \<union> set8_T1_pre y \<Longrightarrow> U1FVars_1' t (pu p) \<subseteq> FVars_T11 t \<union> PFVars_1 p \<union> avoiding_set1) \<Longrightarrow>
+  (\<And>t pu p. (t, pu) \<in> set9_T1_pre y \<union> set10_T1_pre y \<Longrightarrow> U2FVars_1' t (pu p) \<subseteq> FVars_T21 t \<union> PFVars_1 p \<union> avoiding_set1) \<Longrightarrow>
+  U1FVars_1' (raw_T1_ctor (map_T1_pre id id id id id id fst fst fst fst y)) (U1ctor' y p) \<subseteq> FVars_T11 (raw_T1_ctor (map_T1_pre id id id id id id fst fst fst fst y)) \<union> PFVars_1 p \<union> avoiding_set1"
+  "set6_T1_pre (y::(_, _, 'a::{var_T1_pre,var_T2_pre}, 'b, _, _, _, _, _, _) T1_pre) \<inter> (PFVars_2 p \<union> avoiding_set2) = {} \<Longrightarrow>
+  (\<And>t pu p. (t, pu) \<in> set7_T1_pre y \<union> set8_T1_pre y \<Longrightarrow> U1FVars_2' t (pu p) \<subseteq> FVars_T12 t \<union> PFVars_2 p \<union> avoiding_set2) \<Longrightarrow>
+  (\<And>t pu p. (t, pu) \<in> set9_T1_pre y \<union> set10_T1_pre y \<Longrightarrow> U2FVars_2' t (pu p) \<subseteq> FVars_T22 t \<union> PFVars_2 p \<union> avoiding_set2) \<Longrightarrow>
+  U1FVars_2' (raw_T1_ctor (map_T1_pre id id id id id id fst fst fst fst y)) (U1ctor' y p) \<subseteq> FVars_T12 (raw_T1_ctor (map_T1_pre id id id id id id fst fst fst fst y)) \<union> PFVars_2 p \<union> avoiding_set2"
+  apply -
+  subgoal
+    apply (unfold U1FVars_1'_def U1FVars_2'_def U2FVars_1'_def U2FVars_2'_def U1ctor'_def U2ctor'_def FVars_def2s T1.TT_abs_ctors)
+    apply (subst T1_pre.map_comp T2_pre.map_comp, (rule supp_id_bound bij_id)+)
+    apply (unfold fst_comp_map_prod)
+    apply (subst T1_pre.map_comp[symmetric] T2_pre.map_comp[symmetric], (rule supp_id_bound bij_id)+)
+    apply (rule iffD2[OF arg_cong2[OF refl, of _ _ "(\<subseteq>)"]])
+     apply (subst T1_pre.map_comp T2_pre.map_comp, (rule supp_id_bound bij_id)+)
+     apply (unfold fst_comp_map_prod)
+    apply (subst T1_pre.map_comp[symmetric] T2_pre.map_comp[symmetric], (rule supp_id_bound bij_id)+)
+     apply (rule refl)
+    apply (rule U1FVars_subsets U2FVars_subsets)
+        apply (subst T1_pre.set_map T2_pre.set_map, (rule supp_id_bound bij_id)+)
+        apply (unfold image_id image_Un[symmetric])
+        apply assumption
+      (* ALLGOALS *)
+      apply ((subst T1_pre.set_map T2_pre.set_map, (rule supp_id_bound bij_id)+)+, unfold image_id)?
+     apply (subst (asm) T1_pre.set_map T2_pre.set_map, (rule supp_id_bound bij_id)+)+
+     apply (unfold image_Un[symmetric])
+       apply (drule exists_map_prod_id)
+       apply (erule exE)
+       apply (erule conjE)
+       apply hypsubst
+    apply assumption
+    (* copied from above *)
+      apply ((subst T1_pre.set_map T2_pre.set_map, (rule supp_id_bound bij_id)+)+, unfold image_id)?
+     apply (subst (asm) T1_pre.set_map T2_pre.set_map, (rule supp_id_bound bij_id)+)+
+     apply (unfold image_Un[symmetric])
+       apply (drule exists_map_prod_id)
+       apply (erule exE)
+       apply (erule conjE)
+       apply hypsubst
+    apply assumption
+    done
+
+  (* copied from above *)
+subgoal
+    apply (unfold U1FVars_1'_def U1FVars_2'_def U2FVars_1'_def U2FVars_2'_def U1ctor'_def U2ctor'_def FVars_def2s T1.TT_abs_ctors)
+    apply (subst T1_pre.map_comp T2_pre.map_comp, (rule supp_id_bound bij_id)+)
+    apply (unfold fst_comp_map_prod)
+    apply (subst T1_pre.map_comp[symmetric] T2_pre.map_comp[symmetric], (rule supp_id_bound bij_id)+)
+    apply (rule iffD2[OF arg_cong2[OF refl, of _ _ "(\<subseteq>)"]])
+     apply (subst T1_pre.map_comp T2_pre.map_comp, (rule supp_id_bound bij_id)+)
+     apply (unfold fst_comp_map_prod)
+    apply (subst T1_pre.map_comp[symmetric] T2_pre.map_comp[symmetric], (rule supp_id_bound bij_id)+)
+     apply (rule refl)
+    apply (rule U1FVars_subsets U2FVars_subsets)
+        apply (subst T1_pre.set_map T2_pre.set_map, (rule supp_id_bound bij_id)+)
+        apply (unfold image_id image_Un[symmetric])
+        apply assumption
+      (* ALLGOALS *)
+      apply ((subst T1_pre.set_map T2_pre.set_map, (rule supp_id_bound bij_id)+)+, unfold image_id)?
+     apply (subst (asm) T1_pre.set_map T2_pre.set_map, (rule supp_id_bound bij_id)+)+
+     apply (unfold image_Un[symmetric])
+       apply (drule exists_map_prod_id)
+       apply (erule exE)
+       apply (erule conjE)
+       apply hypsubst
+    apply assumption
+    (* copied from above *)
+      apply ((subst T1_pre.set_map T2_pre.set_map, (rule supp_id_bound bij_id)+)+, unfold image_id)?
+     apply (subst (asm) T1_pre.set_map T2_pre.set_map, (rule supp_id_bound bij_id)+)+
+     apply (unfold image_Un[symmetric])
+       apply (drule exists_map_prod_id)
+       apply (erule exE)
+       apply (erule conjE)
+       apply hypsubst
+    apply assumption
+    done
+  done
+
+lemma U2FVars'_subsets: "set5_T2_pre (y2::(_, _, 'a::{var_T1_pre,var_T2_pre}, 'b, _, _, _, _, _, _) T2_pre) \<inter> (PFVars_1 p \<union> avoiding_set1) = {} \<Longrightarrow>
+  (\<And>t pu p. (t, pu) \<in> set7_T2_pre y2 \<union> set8_T2_pre y2 \<Longrightarrow> U1FVars_1' t (pu p) \<subseteq> FVars_T11 t \<union> PFVars_1 p \<union> avoiding_set1) \<Longrightarrow>
+  (\<And>t pu p. (t, pu) \<in> set9_T2_pre y2 \<union> set10_T2_pre y2 \<Longrightarrow> U2FVars_1' t (pu p) \<subseteq> FVars_T21 t \<union> PFVars_1 p \<union> avoiding_set1) \<Longrightarrow>
+  U2FVars_1' (raw_T2_ctor (map_T2_pre id id id id id id fst fst fst fst y2)) (U2ctor' y2 p) \<subseteq> FVars_T21 (raw_T2_ctor (map_T2_pre id id id id id id fst fst fst fst y2)) \<union> PFVars_1 p \<union> avoiding_set1"
+ "set6_T2_pre y2 \<inter> (PFVars_2 p \<union> avoiding_set2) = {} \<Longrightarrow>
+  (\<And>t pu p. (t, pu) \<in> set7_T2_pre y2 \<union> set8_T2_pre y2 \<Longrightarrow> U1FVars_2' t (pu p) \<subseteq> FVars_T12 t \<union> PFVars_2 p \<union> avoiding_set2) \<Longrightarrow>
+  (\<And>t pu p. (t, pu) \<in> set9_T2_pre y2 \<union> set10_T2_pre y2 \<Longrightarrow> U2FVars_2' t (pu p) \<subseteq> FVars_T22 t \<union> PFVars_2 p \<union> avoiding_set2) \<Longrightarrow>
+  U2FVars_2' (raw_T2_ctor (map_T2_pre id id id id id id fst fst fst fst y2)) (U2ctor' y2 p) \<subseteq> FVars_T22 (raw_T2_ctor (map_T2_pre id id id id id id fst fst fst fst y2)) \<union> PFVars_2 p \<union> avoiding_set2"
+  (* same tactic as above *)
+  apply -
+  subgoal
+    apply (unfold U1FVars_1'_def U1FVars_2'_def U2FVars_1'_def U2FVars_2'_def U1ctor'_def U2ctor'_def FVars_def2s T1.TT_abs_ctors)
+    apply (subst T1_pre.map_comp T2_pre.map_comp, (rule supp_id_bound bij_id)+)
+    apply (unfold fst_comp_map_prod)
+    apply (subst T1_pre.map_comp[symmetric] T2_pre.map_comp[symmetric], (rule supp_id_bound bij_id)+)
+    apply (rule iffD2[OF arg_cong2[OF refl, of _ _ "(\<subseteq>)"]])
+     apply (subst T1_pre.map_comp T2_pre.map_comp, (rule supp_id_bound bij_id)+)
+     apply (unfold fst_comp_map_prod)
+    apply (subst T1_pre.map_comp[symmetric] T2_pre.map_comp[symmetric], (rule supp_id_bound bij_id)+)
+     apply (rule refl)
+    apply (rule U1FVars_subsets U2FVars_subsets)
+        apply (subst T1_pre.set_map T2_pre.set_map, (rule supp_id_bound bij_id)+)
+        apply (unfold image_id image_Un[symmetric])
+        apply assumption
+      (* ALLGOALS *)
+      apply ((subst T1_pre.set_map T2_pre.set_map, (rule supp_id_bound bij_id)+)+, unfold image_id)?
+     apply (subst (asm) T1_pre.set_map T2_pre.set_map, (rule supp_id_bound bij_id)+)+
+     apply (unfold image_Un[symmetric])
+       apply (drule exists_map_prod_id)
+       apply (erule exE)
+       apply (erule conjE)
+       apply hypsubst
+    apply assumption
+    (* copied from above *)
+      apply ((subst T1_pre.set_map T2_pre.set_map, (rule supp_id_bound bij_id)+)+, unfold image_id)?
+     apply (subst (asm) T1_pre.set_map T2_pre.set_map, (rule supp_id_bound bij_id)+)+
+     apply (unfold image_Un[symmetric])
+       apply (drule exists_map_prod_id)
+       apply (erule exE)
+       apply (erule conjE)
+       apply hypsubst
+    apply assumption
+    done
+
+  (* copied from above *)
+subgoal
+    apply (unfold U1FVars_1'_def U1FVars_2'_def U2FVars_1'_def U2FVars_2'_def U1ctor'_def U2ctor'_def FVars_def2s T1.TT_abs_ctors)
+    apply (subst T1_pre.map_comp T2_pre.map_comp, (rule supp_id_bound bij_id)+)
+    apply (unfold fst_comp_map_prod)
+    apply (subst T1_pre.map_comp[symmetric] T2_pre.map_comp[symmetric], (rule supp_id_bound bij_id)+)
+    apply (rule iffD2[OF arg_cong2[OF refl, of _ _ "(\<subseteq>)"]])
+     apply (subst T1_pre.map_comp T2_pre.map_comp, (rule supp_id_bound bij_id)+)
+     apply (unfold fst_comp_map_prod)
+    apply (subst T1_pre.map_comp[symmetric] T2_pre.map_comp[symmetric], (rule supp_id_bound bij_id)+)
+     apply (rule refl)
+    apply (rule U1FVars_subsets U2FVars_subsets)
+        apply (subst T1_pre.set_map T2_pre.set_map, (rule supp_id_bound bij_id)+)
+        apply (unfold image_id image_Un[symmetric])
+        apply assumption
+      (* ALLGOALS *)
+      apply ((subst T1_pre.set_map T2_pre.set_map, (rule supp_id_bound bij_id)+)+, unfold image_id)?
+     apply (subst (asm) T1_pre.set_map T2_pre.set_map, (rule supp_id_bound bij_id)+)+
+     apply (unfold image_Un[symmetric])
+       apply (drule exists_map_prod_id)
+       apply (erule exE)
+       apply (erule conjE)
+       apply hypsubst
+    apply assumption
+    (* copied from above *)
+      apply ((subst T1_pre.set_map T2_pre.set_map, (rule supp_id_bound bij_id)+)+, unfold image_id)?
+     apply (subst (asm) T1_pre.set_map T2_pre.set_map, (rule supp_id_bound bij_id)+)+
+     apply (unfold image_Un[symmetric])
+       apply (drule exists_map_prod_id)
+       apply (erule exE)
+       apply (erule conjE)
+       apply hypsubst
+    apply assumption
+    done
+  done
+
+lemma Pmap_imsupp_empty:
+  fixes f1::"'var::{var_T1_pre,var_T2_pre} \<Rightarrow> 'var" and f2::"'tyvar::{var_T1_pre,var_T2_pre} \<Rightarrow> 'tyvar"
+  assumes "bij f1" "|supp f1| <o |UNIV::'var set|" "bij f2" "|supp f2| <o |UNIV::'tyvar set|"
+    "imsupp f1 \<inter> PFVars_1 p = {}" "imsupp f2 \<inter> PFVars_2 p = {}"
+  shows "Pmap f1 f2 p = p"
+  apply (rule Pmap_cong_id)
+       apply (rule assms)+
+   apply (erule id_onD[OF imsupp_id_on, rotated], rule assms)+
+  done
+
+lemma U1ctor_rename:
+  fixes f1::"'var::{var_T1_pre,var_T2_pre} \<Rightarrow> 'var" and f2::"'tyvar::{var_T1_pre,var_T2_pre} \<Rightarrow> 'tyvar"
+  assumes "bij f1" "|supp f1| <o |UNIV::'var set|" "bij f2" "|supp f2| <o |UNIV::'tyvar set|"
+  shows
+    "(\<And>t pu p. (t, pu) \<in> set7_T1_pre y \<union> set8_T1_pre y \<Longrightarrow> U1FVars_1 t (pu p) \<subseteq> FFVars_T11 t \<union> PFVars_1 p \<union> avoiding_set1) \<Longrightarrow>
+  (\<And>t pu p. (t, pu) \<in> set9_T1_pre y \<union> set10_T1_pre y \<Longrightarrow> U2FVars_1 t (pu p) \<subseteq> FFVars_T21 t \<union> PFVars_1 p \<union> avoiding_set1) \<Longrightarrow>
+  (\<And>t pu p. (t, pu) \<in> set7_T1_pre y \<union> set8_T1_pre y \<Longrightarrow> U1FVars_2 t (pu p) \<subseteq> FFVars_T12 t \<union> PFVars_2 p \<union> avoiding_set2) \<Longrightarrow>
+  (\<And>t pu p. (t, pu) \<in> set9_T1_pre y \<union> set10_T1_pre y \<Longrightarrow> U2FVars_2 t (pu p) \<subseteq> FFVars_T22 t \<union> PFVars_2 p \<union> avoiding_set2) \<Longrightarrow>
+  imsupp f1 \<inter> (FFVars_T11 (T1_ctor (map_T1_pre id id id id id id fst fst fst fst y)) \<union> PFVars_1 p \<union> avoiding_set1) = {} \<Longrightarrow>
+  imsupp f2 \<inter> (FFVars_T12 (T1_ctor (map_T1_pre id id id id id id fst fst fst fst y)) \<union> PFVars_2 p \<union> avoiding_set2) = {} \<Longrightarrow>
+  f1 ` set5_T1_pre y \<inter> set5_T1_pre y = {} \<Longrightarrow> f2 ` set6_T1_pre y \<inter> set6_T1_pre y = {} \<Longrightarrow>
+  U1ctor y p = U1ctor (map_T1_pre f1 f2 id id f1 f2
+    (\<lambda>(t, pu). (rrename_T1 f1 f2 t, PU1map f1 f2 t pu)) (\<lambda>(t, pu). (rrename_T1 f1 f2 t, PU1map f1 f2 t pu))
+    (\<lambda>(t, pu). (rrename_T2 f1 f2 t, PU2map f1 f2 t pu)) (\<lambda>(t, pu). (rrename_T2 f1 f2 t, PU2map f1 f2 t pu))
+  y) p"
+  apply (rule sym)
+  apply (rule trans)
+  apply (rule trans)
+   apply (rule arg_cong2[OF refl, of _ _ U1ctor] arg_cong2[OF refl, of _ _ U2ctor])
+   apply (rule Pmap_imsupp_empty[symmetric, OF assms(1-4)])
+    apply ((unfold Int_Un_distrib Un_empty)[1], (erule conjE)+, assumption)+
+  apply (unfold PU1map_def PU2map_def)
+   apply (rule U1map_Uctor[symmetric] U2map_Uctor[symmetric])
+      apply (rule assms)+
+  apply (rule U1map_cong_id U2map_cong_id)
+  apply (rule assms)+
+(* ALLGOALS *)
+   apply (drule set_rev_mp)
+    apply (rule U1FVars_subsets U2FVars_subsets)
+      apply (erule Int_subset_empty1[OF Int_Un_emptyI2[OF
+      trans[OF arg_cong2[OF refl Un_assoc[symmetric], of "(\<inter>)"]]
+      ] imsupp_image_subset])
+      apply assumption+
+   apply (erule id_onD[OF imsupp_id_on, rotated], assumption)
+  (* copied from above *)
+   apply (drule set_rev_mp)
+    apply (rule U1FVars_subsets U2FVars_subsets)
+      apply (erule Int_subset_empty1[OF Int_Un_emptyI2[OF
+      trans[OF arg_cong2[OF refl Un_assoc[symmetric], of "(\<inter>)"]]
+      ] imsupp_image_subset])
+      apply assumption+
+  apply (erule id_onD[OF imsupp_id_on, rotated], assumption)
+  done
+lemma U2ctor_rename:
+  fixes f1::"'var::{var_T1_pre,var_T2_pre} \<Rightarrow> 'var" and f2::"'tyvar::{var_T1_pre,var_T2_pre} \<Rightarrow> 'tyvar"
+  assumes "bij f1" "|supp f1| <o |UNIV::'var set|" "bij f2" "|supp f2| <o |UNIV::'tyvar set|"
+  shows
+    "(\<And>t pu p. (t, pu) \<in> set7_T2_pre y \<union> set8_T2_pre y \<Longrightarrow> U1FVars_1 t (pu p) \<subseteq> FFVars_T11 t \<union> PFVars_1 p \<union> avoiding_set1) \<Longrightarrow>
+  (\<And>t pu p. (t, pu) \<in> set9_T2_pre y \<union> set10_T2_pre y \<Longrightarrow> U2FVars_1 t (pu p) \<subseteq> FFVars_T21 t \<union> PFVars_1 p \<union> avoiding_set1) \<Longrightarrow>
+  (\<And>t pu p. (t, pu) \<in> set7_T2_pre y \<union> set8_T2_pre y \<Longrightarrow> U1FVars_2 t (pu p) \<subseteq> FFVars_T12 t \<union> PFVars_2 p \<union> avoiding_set2) \<Longrightarrow>
+  (\<And>t pu p. (t, pu) \<in> set9_T2_pre y \<union> set10_T2_pre y \<Longrightarrow> U2FVars_2 t (pu p) \<subseteq> FFVars_T22 t \<union> PFVars_2 p \<union> avoiding_set2) \<Longrightarrow>
+  imsupp f1 \<inter> (FFVars_T21 (T2_ctor (map_T2_pre id id id id id id fst fst fst fst y)) \<union> PFVars_1 p \<union> avoiding_set1) = {} \<Longrightarrow>
+  imsupp f2 \<inter> (FFVars_T22 (T2_ctor (map_T2_pre id id id id id id fst fst fst fst y)) \<union> PFVars_2 p \<union> avoiding_set2) = {} \<Longrightarrow>
+  f1 ` set5_T2_pre y \<inter> set5_T2_pre y = {} \<Longrightarrow> f2 ` set6_T2_pre y \<inter> set6_T2_pre y = {} \<Longrightarrow>
+  U2ctor y p = U2ctor (map_T2_pre f1 f2 id id f1 f2
+    (\<lambda>(t, pu). (rrename_T1 f1 f2 t, PU1map f1 f2 t pu)) (\<lambda>(t, pu). (rrename_T1 f1 f2 t, PU1map f1 f2 t pu))
+    (\<lambda>(t, pu). (rrename_T2 f1 f2 t, PU2map f1 f2 t pu)) (\<lambda>(t, pu). (rrename_T2 f1 f2 t, PU2map f1 f2 t pu))
+  y) p"
+(* same tactic as above *)
+apply (rule sym)
+  apply (rule trans)
+  apply (rule trans)
+   apply (rule arg_cong2[OF refl, of _ _ U1ctor] arg_cong2[OF refl, of _ _ U2ctor])
+   apply (rule Pmap_imsupp_empty[symmetric, OF assms(1-4)])
+    apply ((unfold Int_Un_distrib Un_empty)[1], (erule conjE)+, assumption)+
+  apply (unfold PU1map_def PU2map_def)
+   apply (rule U1map_Uctor[symmetric] U2map_Uctor[symmetric])
+      apply (rule assms)+
+  apply (rule U1map_cong_id U2map_cong_id)
+  apply (rule assms)+
+(* ALLGOALS *)
+   apply (drule set_rev_mp)
+    apply (rule U1FVars_subsets U2FVars_subsets)
+      apply (erule Int_subset_empty1[OF Int_Un_emptyI2[OF
+      trans[OF arg_cong2[OF refl Un_assoc[symmetric], of "(\<inter>)"]]
+      ] imsupp_image_subset])
+      apply assumption+
+   apply (erule id_onD[OF imsupp_id_on, rotated], assumption)
+  (* copied from above *)
+   apply (drule set_rev_mp)
+    apply (rule U1FVars_subsets U2FVars_subsets)
+      apply (erule Int_subset_empty1[OF Int_Un_emptyI2[OF
+      trans[OF arg_cong2[OF refl Un_assoc[symmetric], of "(\<inter>)"]]
+      ] imsupp_image_subset])
+      apply assumption+
+  apply (erule id_onD[OF imsupp_id_on, rotated], assumption)
+  done
 
 end
